extract compile function

compiler/src/FlatToRiscv.v
@@ -32,7 +32,7 @@ Require Import riscv.Utility.
 Require Import compiler.runsToNonDet.
 Require Import compiler.Rem4.
 Require Import compiler.containsProgram.
-
+Require Import compiler.FlatToRiscvDef.
 
 (* TODO remove these three *)
 Require Import riscv.MachineWidth_XLEN.
@@ -82,11 +82,14 @@ Existing Instance State_is_RegisterFile.
 
 
 Module Import FlatToRiscv.
+  Export FlatToRiscvDef.FlatToRiscvDef.
+
   Class parameters := {
+    def_params :> FlatToRiscvDef.parameters;
+
     mword: Set;
     MachineWidth_Inst: MachineWidth mword;
     varMap_Inst: MapFunctions Register mword;
-    actname: Set;
     actname_eq_dec: DecidableEq actname;
     Event: Set;  (* element of the event trace *)
 
@@ -116,15 +119,10 @@ Module Import FlatToRiscv.
       (regToZ_unsigned a) mod 8 = 0 ->
       translate mode (ZToReg 8) a = Return a;
 
-    (* TODO move to bitwidth specifics *)
-    LwXLEN: Register -> Register -> Z -> Instruction;
-    SwXLEN: Register -> Register -> Z -> Instruction;
-
-    compile_ext_call: list Register -> actname -> list Register -> list Instruction;
     max_ext_call_code_size: Z;
     max_ext_call_code_size_nonneg: 0 <= max_ext_call_code_size;
     compile_ext_call_length: forall binds f args,
-      Zlength (compile_ext_call binds f args) <= max_ext_call_code_size;
+        Zlength (compile_ext_call binds f args) <= max_ext_call_code_size;
 
     compile_ext_call_correct: forall initialL action outcome post newPc insts
       (argvars resvars: list Register),
@@ -322,87 +320,6 @@ Section FlatToRiscv1.
   (* Set Printing Projections.
      Uncaught anomaly when stepping through proofs :(
      https://github.com/coq/coq/issues/6257 *)
-
-  Definition compile_op(rd: Register)(op: bopname)(rs1 rs2: Register): list Instruction :=
-    match op with
-    | bopname.add => [[Add rd rs1 rs2]]
-    | bopname.sub => [[Sub rd rs1 rs2]]
-    | bopname.mul => [[Mul rd rs1 rs2]]
-    | bopname.and => [[And rd rs1 rs2]]
-    | bopname.or  => [[Or  rd rs1 rs2]]
-    | bopname.xor => [[Xor rd rs1 rs2]]
-    | bopname.sru => [[Srl rd rs1 rs2]]
-    | bopname.slu => [[Sll rd rs1 rs2]]
-    | bopname.srs => [[Sra rd rs1 rs2]]
-    | bopname.lts => [[Slt rd rs1 rs2]]
-    | bopname.ltu => [[Sltu rd rs1 rs2]]
-    | bopname.eq  => [[Sub rd rs1 rs2; Seqz rd rd]]
-    end.
-
-  Fixpoint compile_lit_rec(byteIndex: nat)(rd rs: Register)(v: Z): list Instruction :=
-    let byte := bitSlice v ((Z.of_nat byteIndex) * 8) ((Z.of_nat byteIndex + 1) * 8) in
-    [[ Addi rd rs byte ]] ++
-    match byteIndex with
-    | S b => [[ Slli rd rd 8]] ++ (compile_lit_rec b rd rd v)
-    | O => [[]]
-    end.
-
-  Fixpoint compile_lit_rec'(byteIndex: nat)(rd rs: Register)(v: Z): list Instruction :=
-    let d := (2 ^ ((Z.of_nat byteIndex) * 8))%Z in
-    let hi := (v / d)%Z in
-    let v' := (v - hi * d)%Z in
-    [[ Addi rd rs hi ]] ++
-    match byteIndex with
-    | S b => [[ Slli rd rd 8]] ++ (compile_lit_rec b rd rd v')
-    | O => [[]]
-    end.
-
-  (*
-  Variable rd: Register.
-  Eval cbv -[Register0] in (compile_lit_rec 7 rd Register0 10000).
-  *)
-
-  Definition compile_lit(rd: Register)(v: Z): list Instruction :=
-    compile_lit_rec 7 rd Register0 v.
-
-  Fixpoint compile_stmt(s: stmt): list (Instruction) :=
-    match s with
-    | SLoad x y => [[LwXLEN x y 0]]
-    | SStore x y => [[SwXLEN x y 0]]
-    | SLit x v => compile_lit x v
-    | SOp x op y z => compile_op x op y z
-    | SSet x y => [[Add x Register0 y]]
-    | SIf cond bThen bElse =>
-        let bThen' := compile_stmt bThen in
-        let bElse' := compile_stmt bElse in
-        (* only works if branch lengths are < 2^12 *)
-        [[Beq cond Register0 ((Zlength bThen' + 2) * 4)]] ++
-        bThen' ++
-        [[Jal Register0 ((Zlength bElse' + 1) * 4)]] ++
-        bElse'
-    | SLoop body1 cond body2 =>
-        let body1' := compile_stmt body1 in
-        let body2' := compile_stmt body2 in
-        (* only works if branch lengths are < 2^12 *)
-        body1' ++
-        [[Beq cond Register0 ((Zlength body2' + 2) * 4)]] ++
-        body2' ++
-        [[Jal Register0 (- (Zlength body1' + 1 + Zlength body2') * 4)]]
-    | SSeq s1 s2 => compile_stmt s1 ++ compile_stmt s2
-    | SSkip => nil
-    | SCall resvars action argvars => nil (* unsupported *)
-    | SInteract resvars action argvars => compile_ext_call resvars action argvars
-    end.
-
-  (*
-  Lemma embed_lit_size: forall v,
-    length (embed_lit v) <= 3.
-  Proof.
-    intros. clear.
-    unfold wXLEN, bitwidth, embed_lit, embed_lit_32, embed_lit_64 in *.
-    destruct Bw; simpl; omega.
-  Qed.
-  *)
 
   Arguments Z.mul: simpl never.
   Arguments Z.add: simpl never.
