compiler/src/FlatToRiscvDef.v
@@ -1,0 +1,110 @@
+Require Import bedrock2.Macros.
+Require Import compiler.FlatImp.
+Require Import Coq.Lists.List.
+Import ListNotations.
+Require Import Coq.ZArith.ZArith.
+Require Import compiler.Op.
+Require Import riscv.Program.
+Require Import riscv.Decode.
+Require Import riscv.PseudoInstructions.
+Require Import riscv.InstructionCoercions.
+Require Import Coq.micromega.Lia.
+Require Import riscv.Utility.
+
+
+Local Open Scope ilist_scope.
+Local Open Scope Z_scope.
+
+Set Implicit Arguments.
+
+Module Import FlatToRiscvDef.
+  Class parameters := {
+    actname: Set;
+    LwXLEN: Register -> Register -> Z -> Instruction;
+    SwXLEN: Register -> Register -> Z -> Instruction;
+    compile_ext_call: list Register -> actname -> list Register -> list Instruction;
+  }.
+End FlatToRiscvDef.
+
+
+Section FlatToRiscv1.
+  Context {p: unique! FlatToRiscvDef.parameters}.
+
+  Instance bopname_params: Basic_bopnames.parameters := {|
+    Basic_bopnames.varname := Register;
+    Basic_bopnames.funcname := Empty_set;
+    Basic_bopnames.actname := actname;
+  |}.
+
+  Definition compile_op(rd: Register)(op: bopname)(rs1 rs2: Register): list Instruction :=
+    match op with
+    | bopname.add => [[Add rd rs1 rs2]]
+    | bopname.sub => [[Sub rd rs1 rs2]]
+    | bopname.mul => [[Mul rd rs1 rs2]]
+    | bopname.and => [[And rd rs1 rs2]]
+    | bopname.or  => [[Or  rd rs1 rs2]]
+    | bopname.xor => [[Xor rd rs1 rs2]]
+    | bopname.sru => [[Srl rd rs1 rs2]]
+    | bopname.slu => [[Sll rd rs1 rs2]]
+    | bopname.srs => [[Sra rd rs1 rs2]]
+    | bopname.lts => [[Slt rd rs1 rs2]]
+    | bopname.ltu => [[Sltu rd rs1 rs2]]
+    | bopname.eq  => [[Sub rd rs1 rs2; Seqz rd rd]]
+    end.
+
+  Fixpoint compile_lit_rec(byteIndex: nat)(rd rs: Register)(v: Z): list Instruction :=
+    let byte := bitSlice v ((Z.of_nat byteIndex) * 8) ((Z.of_nat byteIndex + 1) * 8) in
+    [[ Addi rd rs byte ]] ++
+    match byteIndex with
+    | S b => [[ Slli rd rd 8]] ++ (compile_lit_rec b rd rd v)
+    | O => [[]]
+    end.
+
+  Fixpoint compile_lit_rec'(byteIndex: nat)(rd rs: Register)(v: Z): list Instruction :=
+    let d := (2 ^ ((Z.of_nat byteIndex) * 8))%Z in
+    let hi := (v / d)%Z in
+    let v' := (v - hi * d)%Z in
+    [[ Addi rd rs hi ]] ++
+    match byteIndex with
+    | S b => [[ Slli rd rd 8]] ++ (compile_lit_rec b rd rd v')
+    | O => [[]]
+    end.
+
+  (*
+  Variable rd: Register.
+  Eval cbv -[Register0] in (compile_lit_rec 7 rd Register0 10000).
+  *)
+
+  Definition compile_lit(rd: Register)(v: Z): list Instruction :=
+    compile_lit_rec 7 rd Register0 v.
+
+  Fixpoint compile_stmt(s: stmt): list (Instruction) :=
+    match s with
+    | SLoad x y => [[LwXLEN x y 0]]
+    | SStore x y => [[SwXLEN x y 0]]
+    | SLit x v => compile_lit x v
+    | SOp x op y z => compile_op x op y z
+    | SSet x y => [[Add x Register0 y]]
+    | SIf cond bThen bElse =>
+        let bThen' := compile_stmt bThen in
+        let bElse' := compile_stmt bElse in
+        (* only works if branch lengths are < 2^12 *)
+        [[Beq cond Register0 ((Zlength bThen' + 2) * 4)]] ++
+        bThen' ++
+        [[Jal Register0 ((Zlength bElse' + 1) * 4)]] ++
+        bElse'
+    | SLoop body1 cond body2 =>
+        let body1' := compile_stmt body1 in
+        let body2' := compile_stmt body2 in
+        (* only works if branch lengths are < 2^12 *)
+        body1' ++
+        [[Beq cond Register0 ((Zlength body2' + 2) * 4)]] ++
+        body2' ++
+        [[Jal Register0 (- (Zlength body1' + 1 + Zlength body2') * 4)]]
+    | SSeq s1 s2 => compile_stmt s1 ++ compile_stmt s2
+    | SSkip => nil
+    | SCall resvars action argvars => nil (* unsupported *)
+    | SInteract resvars action argvars => compile_ext_call resvars action argvars
+    end.
+
+End FlatToRiscv1.
